Add second example, more complex
Signed-off-by: Nicolas Iooss <nicolas.iooss_git@polytechnique.org>

identity.v
@@ -39,24 +39,83 @@ Save.
 Definition kstate_id : krivine_env := krivine_state krivine_id KEnv_nil KEnv_nil
 .
 
+Theorem closed_code_id:
+  closed_code O krivine_id.
+Proof.
+  unfold closed_code.
+  exists l_id.
+  elim tau_id.
+  apply conj; trivial.
+  apply closed_id.
+Save.
+
 Theorem correct_id:
   correct_state kstate_id.
 Proof.
   apply correct_env_is_state.
   apply Correct_env; simpl.
-    unfold closed_code.
-    exists l_id.
-    elim tau_id.
-    apply conj; trivial.
-    apply closed_id.
+  apply closed_code_id.
   apply Correct_env_nil.
   apply Correct_env_nil.
 Save.
 
 (** Identity is a final state in krivine machine *)
-Theorem final_step:
+Theorem final_step_id:
   krivine_step kstate_id = kstate_id.
 Proof.
-  unfold kstate_id.
   trivial.
+Save.
+
+
+(** Second example, with apply *)
+Definition l_id2 : lterm := Apply l_id l_id
+.
+Definition krivine_id2 : krivine_code := Push krivine_id krivine_id
+.
+Definition kstate_id2 : krivine_env := krivine_state krivine_id2 KEnv_nil KEnv_nil
+.
+Theorem closed_id2:
+  closed l_id2.
+Proof.
+  unfold closed; unfold l_id2. simpl.
+  auto with arith.
+Save.
+Theorem compile_id2:
+  comp l_id2 = krivine_id2.
+Proof.
+  unfold l_id2. unfold krivine_id2. trivial.
+Save.
+Theorem tau_id2:
+  tau_code krivine_id2 = Some l_id2.
+Proof.
+  unfold l_id2. unfold krivine_id2. trivial.
+Save.
+Theorem closed_code_id2:
+  closed_code O krivine_id2.
+Proof.
+  unfold closed_code.
+  exists l_id2.
+  elim tau_id2.
+  apply conj; trivial.
+  apply closed_id2.
+Save.
+Theorem correct_id2:
+  correct_state kstate_id2.
+Proof.
+  apply correct_env_is_state.
+  apply Correct_env; simpl.
+  apply closed_code_id2.
+  apply Correct_env_nil.
+  apply Correct_env_nil.
+Save.
+
+(** Krivine steps on id2 *)
+Theorem krivine_steps_id2:
+  krivine_step kstate_id2 = krivine_state krivine_id KEnv_nil kstate_id /\
+  krivine_step (krivine_step kstate_id2) =
+    krivine_state (Access 0 Nop) kstate_id KEnv_nil /\
+  krivine_step (krivine_step (krivine_step kstate_id2)) = kstate_id.
+Proof.
+  apply conj; trivial.
+  apply conj; trivial.
 Save.
